isabelle/Chapter13_4_Evaluation.thy
@@ -1,349 +1,170 @@
 theory Chapter13_4_Evaluation
-imports Chapter13_3_PatternMatching
+imports Chapter13_3_Typechecking
 begin
 
+primrec is_val :: "expr => bool"
+where "is_val (Var v) = False"
+    | "is_val Zero = True"
+    | "is_val (Suc e) = is_val e"
+    | "is_val (NatRec et e0 es) = False"
+    | "is_val (Lam t e) = True"
+    | "is_val (Appl e1 e2) = False"
+    | "is_val Triv = True"
+    | "is_val (Pair e1 e2) = (is_val e1 & is_val e2)"
+    | "is_val (ProjL e) = False"
+    | "is_val (ProjR e) = False"
+    | "is_val (Abort t e) = False"
+    | "is_val (Case et el er) = False"
+    | "is_val (InL t1 t2 e) = is_val e"
+    | "is_val (InR t1 t2 e) = is_val e"
+    | "is_val (Fold t e) = True"
+    | "is_val (Rec t e1 e2) = False"
+    | "is_val (Unfold t e) = False"
+    | "is_val (Gen t e1 e2) = True"
+
 inductive eval :: "expr => expr => bool"
-      and eval_rules :: "expr => rule list => expr => bool"
-where esuc [simp]: "eval n n' ==> eval (Succ n) (Succ n')"
-    | eap1 [simp]: "eval e1 e1' ==> eval (Ap e1 e2) (Ap e1' e2)"
-    | eap2 [simp]: "is_val e1 ==> eval e2 e2' ==> eval (Ap e1 e2) (Ap e1 e2')"
-    | eap3 [simp]: "is_val e2 ==> eval (Ap (Lam t b) e2) (safe_subst b e2)"
-    | efix [simp]: "eval (Fix t b) (safe_subst b (Fix t b))"
-    | epa1 [simp]: "eval e1 e1' ==> eval (Pair e1 e2) (Pair e1' e2)"
-    | epa2 [simp]: "is_val e1 ==> eval e2 e2' ==> eval (Pair e1 e2) (Pair e1 e2')"
-    | epl1 [simp]: "eval e e' ==> eval (ProjL e) (ProjL e')"
-    | epl2 [simp]: "is_val e1 ==> is_val e2 ==> eval (ProjL (Pair e1 e2)) e1"
-    | epr1 [simp]: "eval e e' ==> eval (ProjR e) (ProjR e')"
-    | epr2 [simp]: "is_val e1 ==> is_val e2 ==> eval (ProjR (Pair e1 e2)) e2"
-    | eabt [simp]: "eval e e' ==> eval (Abort t e) (Abort t e')"
-    | einl [simp]: "eval e e' ==> eval (InL t t' e) (InL t t' e')"
-    | einr [simp]: "eval e e' ==> eval (InR t t' e) (InR t t' e')"
-    | ecs1 [simp]: "eval e e' ==> eval (Case e t rs) (Case e' t rs)"
-    | ecs2 [simp]: "is_val e ==> eval_rules e rs e' ==> eval (Case e t rs) e'"
-    | ers1 [simp]: "is_val e ==> matches p e = Some s ==> eval_rules e (Rule p e2 # rs) (apply_subst s e2)"
-    | ers2 [simp]: "is_val e ==> matches p e = None ==> eval_rules e rs e' ==> eval_rules e (Rule p e2 # rs) e'"
+where eval_suc [simp]: "eval e e' ==> eval (Suc e) (Suc e')"
+    | eval_natrec_1 [simp]: "eval et et' ==> eval (NatRec et e0 es) (NatRec et e0 es)"
+    | eval_natrec_2 [simp]: "eval (NatRec Zero e0 es) e0"
+    | eval_natrec_3 [simp]: "is_val et ==> 
+            eval (NatRec (Suc et) e0 es) (subst (NatRec et e0 es) (subst et es))"
+    | eval_appl_1 [simp]: "eval e1 e1' ==> eval (Appl e1 e2) (Appl e1' e2)"
+    | eval_appl_2 [simp]: "is_val e1 ==> eval e2 e2' ==> eval (Appl e1 e2) (Appl e1 e2')"
+    | eval_appl_3 [simp]: "is_val e2 ==> eval (Appl (Lam t2 e1) e2) (subst e2 e1)"
+    | eval_pair_1 [simp]: "eval e1 e1' ==> eval (Pair e1 e2) (Pair e1' e2)"
+    | eval_pair_2 [simp]: "is_val e1 ==> eval e2 e2' ==> eval (Pair e1 e2) (Pair e1 e2')"
+    | eval_projl_1 [simp]: "eval e e' ==> eval (ProjL e) (ProjL e')"
+    | eval_projl_2 [simp]: "eval (ProjL (Pair e1 e2)) e1"
+    | eval_projr_1 [simp]: "eval e e' ==> eval (ProjR e) (ProjR e')"
+    | eval_projr_2 [simp]: "eval (ProjR (Pair e1 e2)) e2"
+    | eval_abort [simp]: "eval e e' ==> eval (Abort t e) (Abort t e')"
+    | eval_case_1 [simp]: "eval et et' ==> eval (Case et el er) (Case et el er)"
+    | eval_case_2 [simp]: "is_val e ==> eval (Case (InL t1 t2 e) el er) (subst e el)"
+    | eval_case_3 [simp]: "is_val e ==> eval (Case (InR t1 t2 e) el er) (subst e er)"
+    | eval_inl [simp]: "eval e e' ==> eval (InL t1 t2 e) (InL t1 t2 e')"
+    | eval_inr [simp]: "eval e e' ==> eval (InR t1 t2 e) (InR t1 t2 e')"
+    | eval_rec_1 [simp]: "eval e2 e2' ==> eval (Rec t e1 e2) (Rec t e1 e2')"
+    | eval_rec_2 [simp]: "eval (Rec t e1 (Fold t e2)) (Rec t e1 e2)"
 
-theorem preservation: "eval e e' ==> typecheck env e t ==> typecheck env e' t"
-    and "eval_rules e rs e' ==> typecheck_rules env rs t t' ==> typecheck env e t ==> typecheck env e' t'"
-proof (induction e e' and e rs e' arbitrary: t env and t t' env rule: eval_eval_rules.inducts)
-case esuc
-  thus ?case by auto
-next case (eap1 e1 e1' e2)
-  hence "EX t2. typecheck env e1' (Arr t2 t) & typecheck env e2 t2" by auto
-  thus ?case by auto
-next case (eap2 e1 e2 e2')
-  thus ?case by auto
-next case eap3
-  thus ?case by auto
-next case efix
-  thus ?case by auto
-next case epa1
-  thus ?case by auto
-next case epa2
-  thus ?case by auto
-next case (epl1 e e')
-  hence "!!t2. typecheck env e (Prod t t2) ==> typecheck env e' (Prod t t2)" by simp
-  with epl1 have "EX t2. typecheck env e' (Prod t t2)" by auto
-  thus ?case by auto
-next case epl2
-  thus ?case by auto
-next case (epr1 e e')
-  hence "!!t1. typecheck env e (Prod t1 t) ==> typecheck env e' (Prod t1 t)" by simp
-  with epr1 have "EX t1. typecheck env e' (Prod t1 t)" by auto
-  thus ?case by auto
-next case epr2
-  thus ?case by auto
-next case eabt
-  thus ?case by auto
-next case einl
-  thus ?case by auto
-next case einr
-  thus ?case by auto
-next case (ecs1 e e' t1 rs)
-  hence "typecheck env e t1 & typecheck_rules env rs t1 t" by auto
-  moreover with ecs1 have "typecheck env e' t1" by simp
-  ultimately show ?case by simp
-next case ecs2
-  thus ?case by auto
-next case (ers1 e p s e2 rs)
-  then obtain ts where "types_from_pat p t ts & typecheck (extend_env ts env) e2 t'" by auto
-  moreover with ers1 have "typecheck_subst env s ts" by simp
-  ultimately show ?case by simp
-next case ers2
-  thus ?case by auto
+lemma canonical_nat: "is_val e ==> typecheck gam e Nat ==> 
+          e = Zero | (EX e'. e = Suc e' & typecheck gam e' Nat)"
+by (induction e, auto)
+
+lemma canonical_nat_no_vars: "is_val e ==> typecheck gam e Nat ==> typecheck gam' e Nat"
+by (induction e, auto) 
+
+lemma canonical_arrow: "is_val e ==> typecheck gam e (Arrow t1 t2) ==> 
+              EX e'. e = Lam t1 e' & typecheck (extend gam t1) e' t2"
+by (induction e, auto)
+
+lemma canonical_triv: "is_val e ==> typecheck gam e Unit ==> e = Triv"
+by (induction e, auto)
+
+lemma canonical_pair: "is_val e ==> typecheck gam e (Prod t1 t2) ==> 
+              EX e1 e2. e = Pair e1 e2 & typecheck gam e1 t1 & typecheck gam e2 t2"
+by (induction e, auto)
+
+lemma canonical_void: "is_val e ==> typecheck gam e Void ==> False"
+by (induction e, auto)
+
+lemma canonical_sum: "is_val e ==> typecheck gam e (Sum t1 t2) ==> 
+          (EX e'. e = InL t1 t2 e' & typecheck gam e' t1) | 
+          (EX e'. e = InR t1 t2 e' & typecheck gam e' t2)"
+by (induction e, auto)
+
+lemma canonical_ind: "is_val e ==> typecheck gam e (Ind t) ==> 
+          EX e'. e = Fold t e' & typecheck gam e' (type_subst (Ind t) t)"
+by (induction e, auto)
+
+lemma canonical_coind: "is_val e ==> typecheck gam e (Coind t) ==> 
+          EX e1 e2 t2. e = Gen t e1 e2 & typecheck gam e2 t2 & 
+                       typecheck (extend gam t2) e1 (type_subst t2 t)"
+by (induction e, auto)
+
+theorem preservation: "eval e e' ==> typecheck gam e t ==> typecheck gam e' t"
+proof (induction e e' arbitrary: t rule: eval.induct)
+case eval_suc 
+  thus ?case by fastforce
+next case eval_natrec_1 
+  thus ?case by fastforce
+next case eval_natrec_2 
+  thus ?case by fastforce
+next case (eval_natrec_3 et e0 es)
+  from eval_natrec_3 canonical_nat_no_vars have "typecheck (extend gam t) (subst et es) t" by auto
+  with eval_natrec_3 show ?case by fastforce
+next case eval_appl_1 
+  thus ?case by fastforce
+next case eval_appl_2 
+  thus ?case by fastforce
+next case eval_appl_3 
+  thus ?case by fastforce
+next case eval_pair_1 
+  thus ?case by fastforce
+next case eval_pair_2 
+  thus ?case by fastforce
+next case eval_projl_1 
+  thus ?case by fastforce
+next case eval_projl_2 
+  thus ?case by fastforce
+next case eval_projr_1 
+  thus ?case by fastforce
+next case eval_projr_2 
+  thus ?case by fastforce
+next case eval_abort
+  thus ?case by fastforce
+next case eval_case_1 
+  thus ?case by fastforce
+next case eval_case_2 
+  thus ?case by fastforce
+next case eval_case_3 
+  thus ?case by fastforce
+next case eval_inl
+  thus ?case by fastforce
+next case eval_inr
+  thus ?case by fastforce
+next case eval_rec_1
+  thus ?case by fastforce
 qed
 
-lemma [simp]: "matches p v = None ==> is_val v ==> perfectly_satisfied t (extract_patterns (Rule p e # rs)) ==> 
-                  typecheck env v t ==> EX a. eval_rules v rs a"
-proof (induction t)
-case Nat
-  hence "v = Zero | (EX v'. typecheck env v' Nat & is_val v' & v = Succ v')" by (simp add: canonical_nat)
-  with Nat show ?case
-  proof auto
-    fix z v'
-    assume "(case z of Rule p x => p) = PSucc"
-    then obtain e2 where Z: "z = Rule PSucc e2" by (induction z, auto)
-    assume "is_val v'"
-    hence "!!s p. matches p (Succ v') = Some s ==> eval_rules (Succ v') [Rule p e2] (apply_subst s e2)" by simp
-    hence "matches PSucc (Succ v') = Some [v'] ==> eval_rules (Succ v') [Rule PSucc e2] (apply_subst [v'] e2)" by blast
-    with Z have "eval_rules (Succ v') [z] (apply_subst [v'] e2)" by simp
-    thus "EX a. eval_rules (Succ v') [z] a" by (rule exI)
-  next 
-    fix z
-    assume "(case z of Rule p x => p) = PZero"
-    then obtain e2 where Z: "z = Rule PZero e2" by (induction z, auto)
-    hence "!!s p. matches p Zero = Some s ==> eval_rules Zero [Rule p e2] (apply_subst s e2)" by simp
-    hence "matches PZero Zero = Some [] ==> eval_rules Zero [Rule PZero e2] (apply_subst [] e2)" by blast
-    with Z have "eval_rules Zero [z] e2" by simp
-    thus "EX a. eval_rules Zero [z] a" by (rule exI)
-  qed
-next case (Prod t1 t2)
-  hence "EX e1 e2. v = Pair e1 e2 & typecheck env e1 t1 & typecheck env e2 t2 & is_val e1 & is_val e2" by (simp add: canonical_prod)
-  with Prod show ?case by auto
-next case (Sum t1 t2)
-  hence "(EX e'. v = InL t1 t2 e' & is_val e' & typecheck env e' t1) | (EX e'. v = InR t1 t2 e' & is_val e' & typecheck env e' t2)" by (simp add: canonical_sum)
-  with Sum show ?case
-  proof auto
-    fix z v'
-    assume "(case z of Rule p x => p) = PInR"
-    then obtain e2 where Z: "z = Rule PInR e2" by (induction z, auto)
-    assume "is_val v'"
-    hence "!!s p. matches p (InR t1 t2 v') = Some s ==> eval_rules (InR t1 t2 v') [Rule p e2] (apply_subst s e2)" by simp
-    hence "matches PInR (InR t1 t2 v') = Some [v'] ==> eval_rules (InR t1 t2 v') [Rule PInR e2] (apply_subst [v'] e2)" by blast
-    with Z have "eval_rules (InR t1 t2 v') [z] (apply_subst [v'] e2)" by simp
-    thus "EX a. eval_rules (InR t1 t2 v') [z] a" by (rule exI)
-  next 
-    fix z v'
-    assume "(case z of Rule p x => p) = PInL"
-    then obtain e2 where Z: "z = Rule PInL e2" by (induction z, auto)
-    assume "is_val v'"
-    hence "!!s p. matches p (InL t1 t2 v') = Some s ==> eval_rules (InL t1 t2 v') [Rule p e2] (apply_subst s e2)" by simp
-    hence "matches PInL (InL t1 t2 v') = Some [v'] ==> eval_rules (InL t1 t2 v') [Rule PInL e2] (apply_subst [v'] e2)" by blast
-    with Z have "eval_rules (InL t1 t2 v') [z] (apply_subst [v'] e2)" by simp
-    thus "EX a. eval_rules (InL t1 t2 v') [z] a" by (rule exI)
-  qed
-next case Unit
-  hence "v = Triv" by (simp add: canonical_unit)
-  with Unit show ?case by simp
-next case Void
+theorem progress: "typecheck gam e t ==> gam = empty_env ==> is_val e | (EX e'. eval e e')"
+proof (induction gam e t rule: typecheck.induct)
+case tc_var
   thus ?case by simp
-next case Arr
+next case tc_zero
+  thus ?case by simp
+next case tc_suc
+  thus ?case by (metis eval_suc is_val.simps(3))
+next case tc_natrec
+  thus ?case by (metis eval_natrec_1 eval_natrec_2 eval_natrec_3 is_val.simps(3) canonical_nat)
+next case tc_lam
+  thus ?case by simp
+next case tc_appl
+  thus ?case by (metis eval_appl_1 eval_appl_2 eval_appl_3 canonical_arrow)
+next case tc_triv
+  thus ?case by simp
+next case tc_pair
+  thus ?case by (metis eval_pair_1 eval_pair_2 is_val.simps(8))
+next case tc_projl
+  thus ?case by (metis eval_projl_1 eval_projl_2 canonical_pair)
+next case tc_projr
+  thus ?case by (metis eval_projr_1 eval_projr_2 canonical_pair)
+next case tc_abort
+  thus ?case by (metis eval_abort canonical_void)
+next case tc_case
+  thus ?case 
+  by (metis eval_case_1 eval_case_2 eval_case_3 is_val.simps(13) is_val.simps(14) canonical_sum)
+next case tc_inl
+  thus ?case by (metis eval_inl is_val.simps(13))
+next case tc_inr
+  thus ?case by (metis eval_inr is_val.simps(14))
+next case tc_fold
+  thus ?case by simp
+next case tc_rec
+  thus ?case by simp sorry
+next case tc_unfold
+  thus ?case by simp sorry
+next case tc_gen
   thus ?case by simp
 qed
-
-theorem progress: "typecheck env e t ==> env = empty_map ==> all_matches_complete e ==> is_val e | (EX e'. eval e e')"
-    and "typecheck_rules env rs t1 t ==> check_rules rs ==> is_val v ==> typecheck env v t1 ==> 
-            perfectly_satisfied t1 (extract_patterns rs) ==> EX e'. eval_rules v rs e'"
-    and "typecheck_rule env r t1 t ==> True"
-proof (induction env e t and env rs t1 t arbitrary: and v rule: typecheck_typecheck_rules_typecheck_rule.inducts)
-case tvar
-  thus ?case by auto
-next case tzer
-  thus ?case by simp
-next case (tsuc env n)
-  thus ?case 
-  proof (cases "is_val n", auto)
-    fix x
-    assume "eval n x"
-    hence "eval (Succ n) (Succ x)" by simp
-    thus "EX y. eval (Succ n) y " by auto
-  qed
-next case tlam
-  thus ?case by simp
-next case (tapp env e1 t2 t e2)
-  show ?case
-  proof (cases "is_val e1")
-  case True
-    with tapp have "EX v. e1 = Lam t2 v & typecheck (extend_at env 0 t2) v t" by (simp add: canonical_arr)
-    hence e1_is_lam: "EX v. e1 = Lam t2 v" by auto
-    thus ?thesis 
-    proof (cases "is_val e2")
-    case True
-      with e1_is_lam show ?thesis
-      proof auto
-        fix v
-        assume "is_val e2"
-        hence "eval (Ap (Lam t2 v) e2) (safe_subst v e2)" by simp
-        thus "EX x. eval (Ap (Lam t2 v) e2) x" by auto
-      qed
-    next case False
-      with tapp have "\<exists>a. eval e2 a" by auto
-      thus ?thesis
-      proof auto
-        fix a
-        assume "eval e2 a"
-        moreover from True have "is_val e1" by simp
-        ultimately have "eval (Ap e1 e2) (Ap e1 a)" by simp
-        thus "EX x. eval (Ap e1 e2) x" by auto
-      qed
-    qed
-  next case False
-    with tapp have "\<exists>a. eval e1 a" by auto
-    thus ?thesis
-    proof auto
-      fix a
-      assume "eval e1 a"
-      hence "eval (Ap e1 e2) (Ap a e2)" by simp
-      thus "EX x. eval (Ap e1 e2) x" by auto
-    qed
-  qed
-next case (tfix env t b)
-  def b' == "safe_subst b (Fix t b)"
-  have "eval (Fix t b) b'" by (simp add: b'_def)
-  thus ?case by auto
-next case ttrv
-  thus ?case by simp
-next case (tpar env e1 t1 e2 t2)
-  thus ?case
-  proof (cases "is_val e1")
-  case True
-    hence X: "is_val e1" by simp
-    thus ?thesis
-    proof (cases "is_val e2")
-    case True
-      with X show ?thesis by simp  
-    next case False
-      with tpar have "EX a. eval e2 a" by auto
-      hence "EX a. eval (Pair e1 e2) a"
-      proof auto
-        fix e2'
-        assume "eval e2 e2'"
-        with True have "eval (Pair e1 e2) (Pair e1 e2')" by simp
-        thus "EX a. eval (Pair e1 e2) a" by auto
-      qed
-      thus ?thesis by simp  
-    qed
-  next case False
-    with tpar have "EX a. eval e1 a" by auto
-    hence "EX a. eval (Pair e1 e2) a"
-    proof auto
-      fix e1'
-      assume "eval e1 e1'"
-      hence "eval (Pair e1 e2) (Pair e1' e2)" by simp
-      thus "EX a. eval (Pair e1 e2) a" by auto
-    qed
-    with False show ?thesis by simp
-  qed
-next case (tprl env e t1 t2)
-  thus ?case
-  proof (cases "is_val e")
-  case True
-    with tprl have "EX e1 e2. e = Pair e1 e2 & typecheck env e1 t1 & typecheck env e2 t2 & is_val e1 & is_val e2" by (simp add: canonical_prod)
-    thus ?thesis
-    proof auto
-      fix e1 e2
-      assume "is_val e1"
-         and "is_val e2"
-      hence "eval (ProjL (Pair e1 e2)) e1" by simp
-      thus "EX a. eval (ProjL (Pair e1 e2)) a" by auto
-    qed
-  next case False
-    with tprl have "EX a. eval e a" by auto
-    thus ?thesis
-    proof auto
-      fix a
-      assume "eval e a"
-      hence "eval (ProjL e) (ProjL a)" by simp
-      thus "EX a. eval (ProjL e) a" by auto
-    qed
-  qed
-next case (tprr env e t1 t2)
-  thus ?case
-  proof (cases "is_val e")
-  case True
-    with tprr have "EX e1 e2. e = Pair e1 e2 & typecheck env e1 t1 & typecheck env e2 t2 & is_val e1 & is_val e2" by (simp add: canonical_prod)
-    thus ?thesis
-    proof auto
-      fix e1 e2
-      assume "is_val e1"
-         and "is_val e2"
-      hence "eval (ProjR (Pair e1 e2)) e2" by simp
-      thus "EX a. eval (ProjR (Pair e1 e2)) a" by auto
-    qed
-  next case False
-    with tprr have "EX a. eval e a" by auto
-    thus ?thesis
-    proof auto
-      fix a
-      assume "eval e a"
-      hence "eval (ProjR e) (ProjR a)" by simp
-      thus "EX a. eval (ProjR e) a" by auto
-    qed
-  qed
-next case (tabt env e t)
-  thus ?case
-  proof (cases "is_val e", auto simp add: canonical_void)
-    fix x
-    assume "eval e x"
-    hence "eval (Abort t e) (Abort t x)" by simp
-    thus "EX x. eval (Abort t e) x" by auto
-  qed
-next case (tinl env e t1 t2)
-  thus ?case 
-  proof (cases "is_val e", auto)
-    fix x
-    assume "eval e x"
-    hence "eval (InL t1 t2 e) (InL t1 t2 x)" by simp
-    thus "EX y. eval (InL t1 t2 e) y " by auto
-  qed
-next case (tinr env e t2 t1)
-  thus ?case 
-  proof (cases "is_val e", auto)
-    fix x
-    assume "eval e x"
-    hence "eval (InR t1 t2 e) (InR t1 t2 x)" by simp
-    thus "EX y. eval (InR t1 t2 e) y " by auto
-  qed
-next case (tcse env e t1 rs t2)
-  thus ?case
-  proof (cases "is_val e")
-  case True
-    thus ?thesis
-    proof (cases rs)
-    case Nil
-      with tcse show ?thesis by auto
-    next case (Cons r rs')
-      from tcse have "all_matches_complete e & perfectly_satisfied t1 (extract_patterns rs)" by auto
-      thus ?thesis 
-      proof auto
-        assume "all_matches_complete e" 
-           and "perfectly_satisfied t1 (map (rule_case (%p x. p)) rs)"
-        with tcse True obtain a where "eval_rules e rs a" by auto
-        with True have "eval (Case e t1 rs) a" by simp      
-        thus "EX a. eval (Case e t1 rs) a" by (rule exI)      
-      qed
-    qed
-  next case False
-    with tcse have "EX a. eval e a" by auto
-    then obtain a where "eval e a" by auto
-    hence "eval (Case e t1 rs) (Case a t1 rs)" by simp
-    thus ?thesis by auto
-  qed
-next case tnil
-  thus ?case by auto
-next case (tcns env r t1 t2 rs)
-  thus ?case
-  proof (cases r)
-  case (Rule p e)
-    from tcns Rule obtain ts where "types_from_pat p t1 ts & typecheck (extend_env ts env) e t2" by auto
-    moreover from tcns have "!!s. types_from_pat p t1 ts ==> matches p v = Some s ==> typecheck_subst env s ts" by simp
-    ultimately have X: "!!s. matches p v = Some s ==> typecheck_subst env s ts" by simp
-    thus ?thesis
-    proof (cases "EX s. matches p v = Some s")
-    case False
-      with X have Y: "matches p v = None" by simp
-      with tcns Rule have "EX a. eval_rules v rs a" by simp
-      then obtain a where "eval_rules v rs a" by auto
-      with Y tcns have "eval_rules v (Rule p e # rs) a" by simp
-      with Rule show ?thesis by auto
-    next case True
-      with X obtain s where "matches p v = Some s" by auto
-      with tcns have "eval_rules v (Rule p e # rs) (apply_subst s e)" by simp
-      with Rule show ?thesis by auto
-    qed
-  qed
-next case trul
-  thus ?case by simp
-qed 
 
 end
